compositional_compcert/compiler_correctness_trans.v
@@ -578,72 +578,77 @@ Lemma diagram_injinj: forall
             clos_trans (core_data12 * option C2 * core_data23)
               (sem_compose_ord_eq_eq core_ord12 core_ord23 C2) cd'
               (d12, Some st2, d23)).
-Proof. intros. 
-    destruct (core_diagram12 _ _ _ _ CS1 _ _ _ _ MC12)
-          as [st2' [m2' [d12' [j12' [InjIncr12 [InjSep12 [MC12' Y]]]]]]]; clear core_diagram12.
-    assert (ZZ: corestep_plus Sem2 Genv2 st2 m2 st2' m2' \/
-                 (st2,m2) = (st2',m2') /\ core_ord12 d12' d12).
-       destruct Y. auto.
-       destruct H.
-       destruct H. destruct x.
-       right. split; auto.
-       left. exists x; auto.
-    clear Y. destruct ZZ as [CS2 | [CS2 ord12']].
+Proof. 
+  intros. 
+  destruct (core_diagram12 _ _ _ _ CS1 _ _ _ _ MC12)
+    as [st2' [m2' [d12' [j12' [InjIncr12 [InjSep12 [MC12' Y]]]]]]]; clear core_diagram12.
+  assert (ZZ: corestep_plus Sem2 Genv2 st2 m2 st2' m2' \/
+    (st2,m2) = (st2',m2') /\ core_ord12 d12' d12).
+  destruct Y. auto.
+  destruct H.
+  destruct H. destruct x.
+  right. split; auto.
+  left. exists x; auto.
+  clear Y. destruct ZZ as [CS2 | [CS2 ord12']].
  (*case1*) 
-    destruct CS2.
-    clear CS1. 
-    cut (exists st3' : C3,  exists m3' : mem, exists d23':core_data23, exists j23' : meminj, 
-                  inject_incr j23 j23' /\ inject_separated j23 j23' m2 m3 /\
-                   match_core23 d23' j23' st2' m2' st3' m3' /\
-                   (corestep_plus Sem3 Genv3 st3 m3 st3' m3' \/
-                      (corestep_star Sem3 Genv3 st3 m3 st3' m3' /\
-                        clos_trans (core_data12 * option C2 * core_data23)
-                           (sem_compose_ord_eq_eq core_ord12 core_ord23 C2) (d12', Some st2', d23')
-                          (d12, Some st2, d23)))).
-           intros XX; destruct XX as [st3' [m3' [d23' [j23' [InjIncr23 [InjSep23 [MC23' ZZ]]]]]]].
-           exists st3'. exists m3'. exists (d12', Some st2', d23'). exists (compose_meminj j12' j23').
-           split. eapply compose_meminj_inject_incr. apply InjIncr12. apply InjIncr23. 
-           split. eapply compose_meminj_inject_separated. apply InjSep12. apply InjSep23. assumption. assumption.
-                                 eapply (MatchHyp12 _ _ _ _ _ _ MC12).
-                                 eapply (MatchHyp23 _ _ _ _ _ _ MC23).
-           split. exists st2'. exists m2'. exists j12'. exists j23'. auto.
-          apply ZZ.
-   clear MC12 InjIncr12 InjSep12 MC12' MatchHyp12. clear st1 m1 st1' m1' j12 j12'. clear G1 C1 D1 Sem1 match_core12 Genv1.
-
-    revert j23 d23 st2 m2 st3 m3 H MC23. 
-    induction x; intros. 
-      (*base case*) simpl in H.
-          destruct H as [c2 [m2'' [? ?]]].
-          inv H0.
-          destruct (core_diagram23 _ _ _ _ H _ _ _ _ MC23) as [st3' [m3' [d23' [j23' [InjInc23 [InjSep23 [? ?]]]]]]].
-          exists st3'. exists m3'. exists d23'. exists j23'. 
-          split; trivial.
-          split; trivial.
-          split; trivial.
-          destruct H1. left; assumption.
-          destruct H1. right. split; trivial.
-          apply t_step. constructor 2. apply H2.
-     (*inductive case*)
-           remember (S x) as x'. simpl in H.
-           destruct H as [st2'' [m2'' [? ?]]]. subst x'.
-           destruct (core_diagram23 _ _ _ _  H _ _ _ _ MC23) as [c3' [m3' [d23' [j23' [InjInc23 [InjSep23 [? ?]]]]]]]. clear core_diagram23.
-           specialize (IHx j23' d23' _ _ c3' m3' H0 H1).
-           destruct IHx as [c3'' [m3'' [d23'' [j23'' [InjIncr' [InjSep' [MC' XX]]]]]]].
-           exists c3''. exists m3''. exists d23''. exists j23''.
-           split. eapply inject_incr_trans. apply InjInc23. apply InjIncr'.
-           split. clear MC' H1. intros b; intros.
-                     remember (j23' b).
-                     destruct o; apply eq_sym in Heqo. 
-                          destruct p. specialize (InjIncr' _ _ _ Heqo). rewrite InjIncr' in H3. inv H3.
-                          destruct (InjSep23 _ _ _ H1 Heqo). split; trivial.
-                     destruct (InjSep' _ _ _ Heqo H3).
-                        split; intros N.
-                             apply H4. apply corestep_fwd in H. apply H. apply N.
-                             apply H5. destruct H2 as [H2 | [H2 _]].
-                                    apply corestep_plus_fwd in H2. apply H2. apply N.
-                                    apply corestep_star_fwd in H2. apply H2. apply N.                      
-           split. apply MC'.
-           destruct H2; destruct XX.
+  destruct CS2.
+  clear CS1. 
+  cut (exists st3' : C3,  exists m3' : mem, exists d23':core_data23, exists j23' : meminj, 
+    inject_incr j23 j23' /\ inject_separated j23 j23' m2 m3 /\
+    match_core23 d23' j23' st2' m2' st3' m3' /\
+    (corestep_plus Sem3 Genv3 st3 m3 st3' m3' \/
+      (corestep_star Sem3 Genv3 st3 m3 st3' m3' /\
+        clos_trans (core_data12 * option C2 * core_data23)
+        (sem_compose_ord_eq_eq core_ord12 core_ord23 C2) (d12', Some st2', d23')
+        (d12, Some st2, d23)))).
+  intros XX; destruct XX as [st3' [m3' [d23' [j23' [InjIncr23 [InjSep23 [MC23' ZZ]]]]]]].
+  exists st3'. exists m3'. exists (d12', Some st2', d23'). exists (compose_meminj j12' j23').
+  split. eapply compose_meminj_inject_incr. apply InjIncr12. apply InjIncr23. 
+  split. eapply compose_meminj_inject_separated. apply InjSep12. apply InjSep23. 
+  assumption. assumption.
+    eapply (MatchHyp12 _ _ _ _ _ _ MC12).
+    eapply (MatchHyp23 _ _ _ _ _ _ MC23).
+    split. exists st2'. exists m2'. exists j12'. exists j23'. auto.
+    apply ZZ.
+  clear MC12 InjIncr12 InjSep12 MC12' MatchHyp12. 
+  clear st1 m1 st1' m1' j12 j12'. 
+  clear G1 C1 D1 Sem1 match_core12 Genv1.
+  revert j23 d23 st2 m2 st3 m3 H MC23. 
+  induction x; intros. 
+   (*base case*) simpl in H.
+    destruct H as [c2 [m2'' [? ?]]].
+    inv H0.
+    destruct (core_diagram23 _ _ _ _ H _ _ _ _ MC23) 
+      as [st3' [m3' [d23' [j23' [InjInc23 [InjSep23 [? ?]]]]]]].
+    exists st3'. exists m3'. exists d23'. exists j23'. 
+    split; trivial.
+    split; trivial.
+    split; trivial.
+    destruct H1. left; assumption.
+    destruct H1. right. split; trivial.
+    apply t_step. constructor 2. apply H2.
+   (*inductive case*)
+    remember (S x) as x'. simpl in H.
+    destruct H as [st2'' [m2'' [? ?]]]. subst x'.
+    destruct (core_diagram23 _ _ _ _  H _ _ _ _ MC23) 
+      as [c3' [m3' [d23' [j23' [InjInc23 [InjSep23 [? ?]]]]]]]. clear core_diagram23.
+    specialize (IHx j23' d23' _ _ c3' m3' H0 H1).
+    destruct IHx as [c3'' [m3'' [d23'' [j23'' [InjIncr' [InjSep' [MC' XX]]]]]]].
+    exists c3''. exists m3''. exists d23''. exists j23''.
+    split. eapply inject_incr_trans. apply InjInc23. apply InjIncr'.
+    split. clear MC' H1. intros b; intros.
+    remember (j23' b).
+    destruct o; apply eq_sym in Heqo. 
+    destruct p. specialize (InjIncr' _ _ _ Heqo). rewrite InjIncr' in H3. inv H3.
+    destruct (InjSep23 _ _ _ H1 Heqo). split; trivial.
+    destruct (InjSep' _ _ _ Heqo H3).
+    split; intros N.
+    apply H4. apply corestep_fwd in H. apply H. apply N.
+    apply H5. destruct H2 as [H2 | [H2 _]].
+    apply corestep_plus_fwd in H2. apply H2. apply N.
+    apply corestep_star_fwd in H2. apply H2. apply N.                      
+    split. apply MC'.
+    destruct H2; destruct XX.
            (*1/4*)
               left. destruct H2 as [n1 ?]. destruct H3 as [n2 ?].
                       exists (n1 + S n2)%nat.
@@ -671,210 +676,179 @@ Proof. intros.
               apply t_step.
               constructor 2. apply H4.
   (*case 2*)
-    inv CS2.
-    exists st3. exists m3. exists (d12',Some st2',d23). exists  (compose_meminj j12' j23). 
-    split. eapply compose_meminj_inject_incr.  assumption. apply inject_incr_refl.
-    split. eapply compose_meminj_inject_separated. eassumption.
-                apply inject_separated_same_meminj. 
-                assumption. apply inject_incr_refl.
-                eapply (MatchHyp12 _ _ _ _ _ _ MC12).
-                eapply (MatchHyp23 _ _ _ _ _ _ MC23).
-    split. exists st2'. exists m2'. exists j12'. exists j23. auto.
-    right. split. exists O. simpl; auto.
-                       apply t_step. constructor 1; auto.
+   inv CS2.
+   exists st3. exists m3. exists (d12',Some st2',d23). exists  (compose_meminj j12' j23). 
+   split. eapply compose_meminj_inject_incr.  assumption. apply inject_incr_refl.
+   split. eapply compose_meminj_inject_separated. eassumption.
+   apply inject_separated_same_meminj. 
+   assumption. apply inject_incr_refl.
+   eapply (MatchHyp12 _ _ _ _ _ _ MC12).
+   eapply (MatchHyp23 _ _ _ _ _ _ MC23).
+   split. exists st2'. exists m2'. exists j12'. exists j23. auto.
+   right. split. exists O. simpl; auto.
+   apply t_step. constructor 1; auto.
 Qed.
 
 Context {F1 C1 V1 F2 C2 V2 F3 C3 V3} 
-       (I :forall F C V : Type, CoreSemantics (Genv.t F V) C mem (list (ident * globdef F V)) -> AST.program F V -> Prop)
-       (Sem1 : CoreSemantics (Genv.t F1 V1) C1 mem (list (ident * globdef F1 V1)))
-       (Sem2 : CoopCoreSem (Genv.t F2 V2) C2 (list (ident * globdef F2 V2)))
-       (Sem3 : CoopCoreSem (Genv.t F3 V3) C3 (list (ident * globdef F3 V3)))
-       ExternIdents epts12  epts23 entrypoints13
-       (P1 : AST.program F1 V1) (P2 : AST.program F2 V2) (P3 : AST.program F3 V3) 
-       (ePts12_ok : CompilerCorrectness.entryPts_ok P1 P2 ExternIdents epts12)
-       (e12 : prog_main P1 = prog_main P2)
-       (g12: CompilerCorrectness.GenvHyp P1 P2)       
-       (EPC: entrypoints_compose epts12 epts23 entrypoints13)
-       (EXT1: In (prog_main P1, CompilerCorrectness.extern_func main_sig) ExternIdents)
-       (EXT2: In (prog_main P2, CompilerCorrectness.extern_func main_sig) ExternIdents)
-       (i1: I F1 C1 V1 Sem1 P1)
-(*       (Inj_init12 : forall m1 : mem,
-               initial_mem Sem1 (Genv.globalenv P1) m1 (prog_defs P1) ->
-               exists m2 : mem,
-                 initial_mem Sem2 (Genv.globalenv P2) m2 (prog_defs P2) /\
-                 Mem.inject j12 m1 m2)*)
-     (SimInj12 : Coop_forward_simulation_inj.Forward_simulation_inject (list (ident * globdef F1 V1))
-             (list (ident * globdef F2 V2)) Sem1 Sem2 (Genv.globalenv P1) (Genv.globalenv P2) epts12)
-     (SimInj23 : Coop_forward_simulation_inj.Forward_simulation_inject (list (ident * globdef F2 V2))
-             (list (ident * globdef F3 V3)) Sem2 Sem3 (Genv.globalenv P2) (Genv.globalenv P3) epts23).
-(*
-Axiom PO_II: 
-forall  m1 m2 m1' j1 (Minj12 : Mem.inject j1 m1 m2) (Fwd1: mem_forward m1 m1') j2
-                          j' (InjInc: inject_incr (compose_meminj j1 j2) j')  
-                          (UnchLUj:  mem_unchanged_on (loc_unmapped (compose_meminj j1 j2)) m1 m1'),
-exists m2', exists j1', exists j2',  Mem.inject j1' m1' m2' /\ mem_forward m2 m2' /\ j' = compose_meminj j1' j2'.
-*)
+  (I :forall F C V : Type, 
+    CoreSemantics (Genv.t F V) C mem (list (ident * globdef F V)) -> 
+    AST.program F V -> Prop)
+  (Sem1 : CoreSemantics (Genv.t F1 V1) C1 mem (list (ident * globdef F1 V1)))
+  (Sem2 : CoopCoreSem (Genv.t F2 V2) C2 (list (ident * globdef F2 V2)))
+  (Sem3 : CoopCoreSem (Genv.t F3 V3) C3 (list (ident * globdef F3 V3)))
+  ExternIdents epts12  epts23 entrypoints13
+  (P1 : AST.program F1 V1) (P2 : AST.program F2 V2) (P3 : AST.program F3 V3) 
+  (ePts12_ok : CompilerCorrectness.entryPts_ok P1 P2 ExternIdents epts12)
+  (e12 : prog_main P1 = prog_main P2)
+  (g12: CompilerCorrectness.GenvHyp P1 P2)       
+  (EPC: entrypoints_compose epts12 epts23 entrypoints13)
+  (EXT1: In (prog_main P1, CompilerCorrectness.extern_func main_sig) ExternIdents)
+  (EXT2: In (prog_main P2, CompilerCorrectness.extern_func main_sig) ExternIdents)
+  (i1: I F1 C1 V1 Sem1 P1)
+  (SimInj12 : Coop_forward_simulation_inj.Forward_simulation_inject (list (ident * globdef F1 V1))
+    (list (ident * globdef F2 V2)) Sem1 Sem2 (Genv.globalenv P1) (Genv.globalenv P2) epts12)
+  (SimInj23 : Coop_forward_simulation_inj.Forward_simulation_inject (list (ident * globdef F2 V2))
+    (list (ident * globdef F3 V3)) Sem2 Sem3 (Genv.globalenv P2) (Genv.globalenv P3) epts23).
 
-Lemma injinj: Coop_forward_simulation_inj.Forward_simulation_inject (list (ident * globdef F1 V1))
-                                         (list (ident * globdef F3 V3)) Sem1 Sem3 (Genv.globalenv P1)
-                                        (Genv.globalenv P3) entrypoints13.
+Lemma injinj: Coop_forward_simulation_inj.Forward_simulation_inject 
+  (list (ident * globdef F1 V1))
+  (list (ident * globdef F3 V3)) Sem1 Sem3 (Genv.globalenv P1)
+  (Genv.globalenv P3) entrypoints13.
 Proof.
-  destruct SimInj12 as [core_data12 match_core12 core_ord12 core_ord_wf12 match_memwd12 match_validblock12 core_diagram12 
-                        core_initial12 core_halted12 core_at_external12 core_after_external12].  
-  destruct SimInj23 as [core_data23 match_core23 core_ord23 core_ord_wf23  match_memwd23 match_validblock23 core_diagram23 
-                        core_initial23 core_halted23 core_at_external23 core_after_external23].
+  destruct SimInj12 
+    as [core_data12 match_core12 core_ord12 core_ord_wf12 match_memwd12 
+      match_validblock12 core_diagram12 
+      core_initial12 core_halted12 core_at_external12 core_after_external12].  
+  destruct SimInj23 
+    as [core_data23 match_core23 core_ord23 core_ord_wf23  match_memwd23 
+      match_validblock23 core_diagram23 
+      core_initial23 core_halted23 core_at_external23 core_after_external23].
   eapply Coop_forward_simulation_inj.Build_Forward_simulation_inject with
-                 (core_ord := clos_trans _ (sem_compose_ord_eq_eq core_ord12 core_ord23 C2))
-                 (match_state := fun d j c1 m1 c3 m3 => 
-                    match d with (d1,X,d2) => 
-                        exists c2, exists m2, exists j1, exists j2, 
-                           X=Some c2 /\ j = compose_meminj j1 j2 /\
-                           match_core12 d1 j1 c1 m1 c2 m2 /\ match_core23 d2 j2 c2 m2 c3 m3 
-                                                                                     
-                    end).
-            (*well_founded*)
-                 eapply wf_clos_trans. eapply well_founded_sem_compose_ord_eq_eq; assumption.
-            (*match_wd*) intros. rename c2 into c3.  rename m2 into m3. destruct d as [[d12 cc2] d23]. 
-                         destruct H as [c2 [m2 [j12 [j23 [X [J [MC12 MC23]]]]]]]; subst.
-                         split. apply (match_memwd12 _ _ _ _ _ _ MC12).
-                                apply (match_memwd23 _ _ _ _ _ _ MC23).
-            (*match_validblocks*) intros. rename c2 into c3.  rename m2 into m3. destruct d as [[d12 cc2] d23]. 
-                         destruct H as [c2 [m2 [j12 [j23 [X [J [MC12 MC23]]]]]]]; subst.
-                         apply compose_meminjD_Some in H0. 
-                         destruct H0 as [b11 [ofs11 [ofs12 [Hb [Hb1 Hdelta]]]]]. 
-                         split. eapply (match_validblock12 _ _ _ _ _ _ MC12); try eassumption.
-                             eapply (match_validblock23 _ _ _ _ _ _ MC23); try eassumption.
-            (*core_diagram*)
-                 clear core_initial23  core_halted23 core_at_external23 core_after_external23 
-                       core_initial12  core_halted12 core_at_external12 core_after_external12
-                       i1 I core_ord_wf23 core_ord_wf12 EXT2 EXT1 EPC e12 g12 ePts12_ok epts12 
-                       epts23 entrypoints13 (*Inj_init12*) SimInj12 SimInj23.
-                 intros. rename st2 into st3. rename m2 into m3.
-                 destruct cd as [[d12 cc2] d23]. destruct H0 as [st2 [m2 [j12 [j23 [X [? [MC12 MC23]]]]]]]; subst.
-                 eapply (diagram_injinj _ _ _ _ _ _ _ _ _ Sem1 Sem2 Sem3 core_data12 match_core12 _ _ _ 
-                                        core_diagram12 _ _ _ _ core_diagram23 
-                            match_validblock12 match_validblock23); try eassumption.
-           (*initial_core*)
-                 clear core_diagram23  core_halted23 core_at_external23 core_after_external23 
-                       core_diagram12  core_halted12 core_at_external12 core_after_external12.
-                  intros. rename m2 into m3. rename v2 into v3. rename vals2 into vals3. 
-                  rewrite (EPC v1 v3 sig) in H. destruct H as [v2 [EP12 EP23]].
-                  assert (HT: Forall2 Val.has_type vals1 (sig_args sig)). 
-                      eapply forall_valinject_hastype; eassumption.
-                  assert (X: Mem.inject (Mem.flat_inj (Mem.nextblock m1)) m1 m1 /\ 
-                             j = compose_meminj (Mem.flat_inj (Mem.nextblock m1)) j ).
-                      split. apply mem_wd_E. apply H2.  
-                             eapply (meminj_split_flatinjL _ _ _ H1). apply H2.
-                  destruct X as [Flat1 XX]. rewrite XX.
-                  assert (ValInjFlat1 := forall_val_inject_flat _ _ _ H1 _ _ H4).
-                  destruct (core_initial12 _ _ _ EP12 _ _ _ _ _ _ H0 Flat1 H2 H2 ValInjFlat1 HT) as [d12 [c2 [Ini2 MC12]]].
-                  destruct (core_initial23 _ _ _ EP23 _ _ _ _ _ _  Ini2 H1 H2 H3 H4 H5) as [d23 [c3 [Ini3 MC23]]].
-                  exists (d12,Some c2,d23). exists c3. 
-                  split; trivial. 
-                  exists c2. exists m1. exists  (Mem.flat_inj (Mem.nextblock m1)). exists j. 
-                  split; trivial. split; trivial. split; assumption.
-             (*safely_halted*)
-                    intros. rename c2 into c3. rename m2 into m3.  
-                    destruct cd as [[d12 cc2] d23]. destruct H as [c2 [m2 [j12 [j23 [X [Y [MC12 MC23]]]]]]]; subst. 
-                    apply (core_halted12 _ _ _ _ _ _ _ MC12) in H0; try assumption. 
-                    destruct H0 as [v2 [ValsInj12 [SH2 [Minj12 VV2]]]].
-                    apply (core_halted23 _ _ _ _ _ _ _ MC23) in SH2; try assumption. 
-                    destruct SH2 as [v3 [ValsInj23 [SH3 [MInj23 VV3]]]].
-                    exists v3. split. apply (val_inject_compose _ _ _ _ _ ValsInj12 ValsInj23).
-                          split. trivial. 
-                          split. eapply Mem.inject_compose; eassumption.
-                          assumption.
-             (*atexternal*)
-                    intros. rename st2 into st3. rename m2 into m3. 
-                    destruct cd as [[d12 cc2] d23]. 
-                    destruct H as [st2 [m2 [j1 [j2 [Y [J [MC12 MC23]]]]]]]. subst.
-                    apply (core_at_external12 _ _ _ _ _ _ _ _ _ MC12) in H0; try assumption. 
-                      destruct H0 as [MInj12 [PGj1 [vals2 [ValsInj12 [HTVals2 [AtExt2 VV2]]]]]].
-                    apply (core_at_external23 _ _ _ _ _ _ _ _ _ MC23) in AtExt2; try assumption. 
-                      destruct AtExt2 as [MInj23 [PGj2 [vals3 [ValsInj23 [HTVals3 [AtExt3 VV3]]]]]].
-                    split. eapply Mem.inject_compose; eassumption.
-                    split. admit. (*need to prove  meminj_preserves_globals (Genv.globalenv P1) (compose_meminj j1 j2)meminj_preserves_globals (Genv.globalenv P1) j1  and meminj_preserves_globals (Genv.globalenv P2) j2*)  
-                    exists vals3. 
-                    split.  eapply forall_val_inject_compose; eassumption.
-                    split; try assumption.
-                    split; try assumption.
-             (*after_external*) clear core_diagram12 core_initial12 core_halted12 
-                                      core_diagram23 core_initial23 core_halted23. 
-                    intros. rename st2 into st3. rename m2 into m3. rename ret2 into ret3. rename m2' into m3'. 
-                    destruct cd as [[d12 cc2] d23]. 
-                    destruct H0 as [st2 [m2 [j1 [j2 [Y [J [MC12 MC23]]]]]]]. subst.
-                    rename H1 into AtExt1. rename H2 into VV1.
-                    destruct (core_at_external12 _ _ _ _ _ _ _ _ _ MC12 AtExt1 VV1) 
-                               as [MInj12 [PGj1 [vals2 [ValsInj12 [HTVals2 [AtExt2 VV2]]]]]].
-                    destruct (core_at_external23 _ _ _ _ _ _ _ _ _ MC23 AtExt2 VV2) 
-                              as [MInj23 [PGj2 [vals3 [ValsInj23 [HTVals3 [AtExt3 V3V]]]]]].
-                    clear core_at_external12 core_at_external23.
-                    assert (HVals1:  Forall2 Val.has_type vals1 (sig_args ef_sig)). 
-                          eapply forall_valinject_hastype; eassumption.
-                    assert (HRet1: Val.has_type ret1 (proj_sig_res ef_sig)). 
-                          eapply valinject_hastype; eassumption.
-                    assert (mem_wd m1 /\ mem_wd m2). apply (match_memwd12 _ _ _ _ _ _ MC12). destruct H0 as [WD1 WD2].
-                    assert (WD3: mem_wd m3). apply (match_memwd23 _ _ _ _ _ _ MC23).
+    (core_ord := clos_trans _ (sem_compose_ord_eq_eq core_ord12 core_ord23 C2))
+    (match_state := fun d j c1 m1 c3 m3 => 
+      match d with (d1,X,d2) => 
+        exists c2, exists m2, exists j1, exists j2, 
+          X=Some c2 /\ j = compose_meminj j1 j2 /\
+          match_core12 d1 j1 c1 m1 c2 m2 /\ match_core23 d2 j2 c2 m2 c3 m3 
+      end).
+ (*well_founded*)
+  eapply wf_clos_trans. eapply well_founded_sem_compose_ord_eq_eq; assumption.
+ (*match_wd*) intros. rename c2 into c3.  rename m2 into m3. destruct d as [[d12 cc2] d23]. 
+  destruct H as [c2 [m2 [j12 [j23 [X [J [MC12 MC23]]]]]]]; subst.
+  split. apply (match_memwd12 _ _ _ _ _ _ MC12).
+  apply (match_memwd23 _ _ _ _ _ _ MC23).
+ (*match_validblocks*) 
+  intros. rename c2 into c3.  rename m2 into m3. destruct d as [[d12 cc2] d23]. 
+  destruct H as [c2 [m2 [j12 [j23 [X [J [MC12 MC23]]]]]]]; subst.
+  apply compose_meminjD_Some in H0. 
+  destruct H0 as [b11 [ofs11 [ofs12 [Hb [Hb1 Hdelta]]]]]. 
+  split. eapply (match_validblock12 _ _ _ _ _ _ MC12); try eassumption.
+  eapply (match_validblock23 _ _ _ _ _ _ MC23); try eassumption.
+ (*core_diagram*)
+  clear core_initial23  core_halted23 core_at_external23 core_after_external23 
+    core_initial12  core_halted12 core_at_external12 core_after_external12
+    i1 I core_ord_wf23 core_ord_wf12 EXT2 EXT1 EPC e12 g12 ePts12_ok epts12 
+    epts23 entrypoints13 (*Inj_init12*) SimInj12 SimInj23.
+  intros. rename st2 into st3. rename m2 into m3.
+  destruct cd as [[d12 cc2] d23]. destruct H0 as [st2 [m2 [j12 [j23 [X [? [MC12 MC23]]]]]]]; subst.
+  eapply (diagram_injinj _ _ _ _ _ _ _ _ _ Sem1 Sem2 Sem3 core_data12 match_core12 _ _ _ 
+    core_diagram12 _ _ _ _ core_diagram23 
+    match_validblock12 match_validblock23); try eassumption.
+ (*initial_core*)
+  clear core_diagram23  core_halted23 core_at_external23 core_after_external23 
+    core_diagram12  core_halted12 core_at_external12 core_after_external12.
+  intros. rename m2 into m3. rename v2 into v3. rename vals2 into vals3. 
+  rewrite (EPC v1 v3 sig) in H. destruct H as [v2 [EP12 EP23]].
+  assert (HT: Forall2 Val.has_type vals1 (sig_args sig)). 
+  eapply forall_valinject_hastype; eassumption.
+  assert (X: Mem.inject (Mem.flat_inj (Mem.nextblock m1)) m1 m1 /\ 
+    j = compose_meminj (Mem.flat_inj (Mem.nextblock m1)) j ).
+  split. apply mem_wd_E. apply H2.  
+  eapply (meminj_split_flatinjL _ _ _ H1). apply H2.
+  destruct X as [Flat1 XX]. rewrite XX.
+  assert (ValInjFlat1 := forall_val_inject_flat _ _ _ H1 _ _ H4).
+  destruct (core_initial12 _ _ _ EP12 _ _ _ _ _ _ H0 Flat1 H2 H2 ValInjFlat1 HT) 
+    as [d12 [c2 [Ini2 MC12]]].
+  destruct (core_initial23 _ _ _ EP23 _ _ _ _ _ _  Ini2 H1 H2 H3 H4 H5) 
+    as [d23 [c3 [Ini3 MC23]]].
+  exists (d12,Some c2,d23). exists c3. 
+  split; trivial. 
+  exists c2. exists m1. exists  (Mem.flat_inj (Mem.nextblock m1)). exists j. 
+  split; trivial. split; trivial. split; assumption.
+ (*safely_halted*)
+  intros. rename c2 into c3. rename m2 into m3.  
+  destruct cd as [[d12 cc2] d23]. destruct H as [c2 [m2 [j12 [j23 [X [Y [MC12 MC23]]]]]]]; subst. 
+  apply (core_halted12 _ _ _ _ _ _ _ MC12) in H0; try assumption. 
+  destruct H0 as [v2 [ValsInj12 [SH2 [Minj12 VV2]]]].
+  apply (core_halted23 _ _ _ _ _ _ _ MC23) in SH2; try assumption. 
+  destruct SH2 as [v3 [ValsInj23 [SH3 [MInj23 VV3]]]].
+  exists v3. split. apply (val_inject_compose _ _ _ _ _ ValsInj12 ValsInj23).
+  split. trivial. 
+  split. eapply Mem.inject_compose; eassumption.
+  assumption.
+(*atexternal*)
+  intros. rename st2 into st3. rename m2 into m3. 
+  destruct cd as [[d12 cc2] d23]. 
+  destruct H as [st2 [m2 [j1 [j2 [Y [J [MC12 MC23]]]]]]]. subst.
+  apply (core_at_external12 _ _ _ _ _ _ _ _ _ MC12) in H0; try assumption. 
+  destruct H0 as [MInj12 [PGj1 [vals2 [ValsInj12 [HTVals2 [AtExt2 VV2]]]]]].
+  apply (core_at_external23 _ _ _ _ _ _ _ _ _ MC23) in AtExt2; try assumption. 
+  destruct AtExt2 as [MInj23 [PGj2 [vals3 [ValsInj23 [HTVals3 [AtExt3 VV3]]]]]].
+  split. eapply Mem.inject_compose; eassumption.
+  split. 
+  admit. (*TODO: need to prove meminj_preserves_globals (Genv.globalenv P1)
+            (compose_meminj j1 j2)meminj_preserves_globals (Genv.globalenv P1) j1
+            and meminj_preserves_globals (Genv.globalenv P2) j2*)
+  exists vals3. 
+  split.  eapply forall_val_inject_compose; eassumption.
+  split; try assumption.
+  split; try assumption.
+ (*after_external*) clear core_diagram12 core_initial12 core_halted12 
+  core_diagram23 core_initial23 core_halted23. 
+  intros. rename st2 into st3. rename m2 into m3. rename ret2 into ret3. rename m2' into m3'. 
+  destruct cd as [[d12 cc2] d23]. 
+  destruct H0 as [st2 [m2 [j1 [j2 [Y [J [MC12 MC23]]]]]]]. subst.
+  rename H1 into AtExt1. rename H2 into VV1.
+  destruct (core_at_external12 _ _ _ _ _ _ _ _ _ MC12 AtExt1 VV1) 
+   as [MInj12 [PGj1 [vals2 [ValsInj12 [HTVals2 [AtExt2 VV2]]]]]].
+  destruct (core_at_external23 _ _ _ _ _ _ _ _ _ MC23 AtExt2 VV2) 
+   as [MInj23 [PGj2 [vals3 [ValsInj23 [HTVals3 [AtExt3 V3V]]]]]].
+  clear core_at_external12 core_at_external23.
+  assert (HVals1:  Forall2 Val.has_type vals1 (sig_args ef_sig)). 
+  eapply forall_valinject_hastype; eassumption.
+  assert (HRet1: Val.has_type ret1 (proj_sig_res ef_sig)). 
+  eapply valinject_hastype; eassumption.
+  assert (mem_wd m1 /\ mem_wd m2). apply (match_memwd12 _ _ _ _ _ _ MC12). destruct H0 as [WD1 WD2].
+  assert (WD3: mem_wd m3). apply (match_memwd23 _ _ _ _ _ _ MC23).
+  destruct (interpolate_II _ _ _ MInj12 _ H8 _ _ MInj23 _ H10 _ H6 H4 H5 H9 H11 WD1 H13 WD2 WD3 H14)
+    as [m2' [j12' [j23' [X [Incr12 [Incr23 [MInj12' [Fwd2 
+      [MInj23' [Unch22 [Sep12 [Sep23 [Unch222' [Unch2233' WD22']]]]]]]]]]]]]]. 
+  subst.
+  assert (WD2': mem_wd m2'). apply WD22'. apply WD2. 
+  assert (exists ret2, val_inject j12' ret1 ret2 /\ val_inject j23' ret2 ret3 /\
+    Val.has_type ret2 (proj_sig_res ef_sig) /\ val_valid ret2 m2'). 
+  apply val_inject_split in H7. destruct H7 as [ret2 [injRet12 injRet23]]. 
+  exists ret2. split; trivial. split; trivial. 
+  split. eapply valinject_hastype; eassumption.
+  eapply inject_valvalid; eassumption. 
+  destruct H0 as [ret2 [injRet12 [injRet23 [HasTp2 ValV2]]]].
+  assert (Unch111': mem_unchanged_on (loc_unmapped j1) m1 m1').
+  split; intros; apply H9; unfold compose_meminj, loc_unmapped in *. 
+  rewrite H0. trivial. trivial. 
+  intros. specialize (H0 _ H2). rewrite H0. trivial. trivial.
+  specialize (core_after_external12 _ _ j12' _ _ _ _ _ ret1 m1' m2 m2' ret2 _ MInj12 MC12 AtExt1
+    VV1 PGj1 Incr12 Sep12 MInj12' injRet12 H8 Unch111' Fwd2 Unch22 HasTp2 H13 WD2' H15 ValV2).
+  destruct core_after_external12 as [d12' [c1' [c2' [AftExt1 [AftExt2 MC12']]]]].
 
-                    destruct (interpolate_II _ _ _ MInj12 _ H8 _ _ MInj23 _ H10 _ H6 H4 H5 H9 H11 WD1 H13 WD2 WD3 H14)
-                       as [m2' [j12' [j23' [X [Incr12 [Incr23 [MInj12' [Fwd2 [MInj23' [Unch22 [Sep12 [Sep23 [Unch222' [Unch2233' WD22']]]]]]]]]]]]]]. 
-                    subst.
-                    assert (WD2': mem_wd m2'). apply WD22'. apply WD2. 
-                    assert (exists ret2, val_inject j12' ret1 ret2 /\ val_inject j23' ret2 ret3 /\
-                            Val.has_type ret2 (proj_sig_res ef_sig) /\ val_valid ret2 m2'). 
-                        apply val_inject_split in H7. destruct H7 as [ret2 [injRet12 injRet23]]. 
-                        exists ret2. split; trivial. split; trivial. 
-                         split. eapply valinject_hastype; eassumption.
-                         eapply inject_valvalid; eassumption. 
-                    destruct H0 as [ret2 [injRet12 [injRet23 [HasTp2 ValV2]]]].
-                    assert (Unch111': mem_unchanged_on (loc_unmapped j1) m1 m1').
-                       split; intros; apply H9; unfold compose_meminj, loc_unmapped in *. 
-                             rewrite H0. trivial. trivial. 
-                         intros. specialize (H0 _ H2). rewrite H0. trivial. trivial.
-                    specialize (core_after_external12 _ _ j12' _ _ _ _ _ ret1 m1' m2 m2' ret2 _ MInj12 MC12 AtExt1
-                                  VV1 PGj1 Incr12 Sep12 MInj12' injRet12 H8 Unch111' Fwd2 Unch22 HasTp2 H13 WD2' H15 ValV2).
-(*                    assert (ValV2': val_valid ret1 m2'). eapply (extends_valvalid _ _ Ext12'). apply H15. *)
-                    destruct core_after_external12 as [d12' [c1' [c2' [AftExt1 [AftExt2 MC12']]]]].
-
-                    specialize (core_after_external23 _ _ j23' _ _ _ _ vals2 ret2 m2' _ m3' ret3 _ MInj23 MC23 
-                               AtExt2 VV2 PGj2 Incr23 Sep23 MInj23' injRet23 Fwd2 Unch222' H10 Unch2233' H12 WD2'
-                                H14 ValV2 H16).
-                    destruct core_after_external23 as [d23' [cc2' [c3' [AftExt22 [AftExt3 MC23']]]]].
-                    rewrite AftExt22 in AftExt2. inv AftExt2.
-                    exists (d12', Some c2', d23'). exists c1'. exists c3'.
-                    split. assumption.
-                    split. assumption.
-                    exists c2'. exists m2'. exists j12'. exists j23'. auto.
-(*
-                    destruct (core_after_external23 _ j j' _ _ _ _ vals2 ret1 _ _ _ ret3 _ Inj23 
-                              MC23 AtExt2 VV2 PG2 H4 Sep23 Inj23' H7 Fwd2' UnchOn2j H10 UnchOn3 H12)
-                         as [d23' [cc2' [c3' [AftExt22 [AftExt3 MC23']]]]]; try assumption; clear core_after_external23.
-
-                    destruct (PO_II _ _ _ _ MInj12 H8 _ _ H4 H9) as [m2' [j1' [j2' [Minj12' [Fwd2' ZZZ]]]]]. subst.
-                    specialize (core_after_external12 d12 j1 j1' st1 st2 m1 e vals1 ret1 m1' m2 m2').
-admit. *)(*Continue here in injinj_afterexternal
-                    apply val_inject_compose_split in H7. destruct H7 as [ret2 [RetJ12 RetJ23]].
-                    assert (MPG1:meminj_preserves_globals (Genv.globalenv P1) j1). 
-admit. (*meminj_preserves_globals*)
-                    specialize  (core_after_external12 ret2 _ MInj12 MC12 AtExt1). 
-specialize (core_after_external12 d12 j1 _ st1 st2 m1 e vals1 ret1 m1' m2).
-                    destruct (inj_incr_compose_split _ _ _ H3) as [j1' [j2' [Jinc1 [Jinc2 J']]]]. subst. 
-specialize (core_after_external12 cd12 j1 j1' st1 st2 m1 e vals1 ret1 m1' m2 m2').
-                    destruct (pushout_II _ _ j1 MInj12 _ H7 j1') as [m2' [Fwd2 [Ext12' [UnchOn2 X]]]].
-                    destruct (X _ H12) as [UnchOn2j Ext23']; clear X.
-                    destruct (core_after_external12 _ _ _ _ _ _ _ _ ret1 ret1 _ _ _ MC12 H5 AtExt2 
-                            LDVals12 HTVals2 H11 Fwd2 UnchOn2 (Val.lessdef_refl _) Ext12' HRet1) as [c1' [c2' [d12' [AftExt1 [AftExt2 MC12']]]]].
-                    assert (UnchOn3 :  mem_unchanged_on (loc_out_of_reach j m2) m3 m3').
-                        split; intros; eapply H14; trivial.
-                                 eapply extends_loc_out_of_reach; eassumption.
-                                 intros. apply H4 in H17. eapply extends_loc_out_of_reach; eassumption.
-                    specialize (Ext23' _ Inj23 _ H13 H14 _ H7 H8 H9).
-                    assert (Sep23: inject_separated j j' m2 m3).
-                         intros b. intros. destruct (H8 _ _ _ H4 H16). split; trivial. intros N. apply H17.  inv Ext12. unfold Mem.valid_block. rewrite mext_next. apply N.
-                    destruct (core_after_external23 _ j j' _ _ _ _ vals2 ret1 _ _ _ ret3 _ Inj23 MC23 AtExt2 PG2 H7 Sep23 Ext23' H10 Fwd2
-                             UnchOn2j H13 UnchOn3 H15)  as [cc2' [c3' [d23' [AftExt22 [AftExt3 MC23']]]]].
-                    rewrite AftExt22 in AftExt2. inv AftExt2.
-                    exists c1'. exists c3'. exists (d12',d23'). split; trivial. split; trivial. exists c2'. exists m2'.  split; trivial.*)
+  specialize (core_after_external23 _ _ j23' _ _ _ _ vals2 ret2 m2' _ m3' ret3 _ MInj23 MC23 
+    AtExt2 VV2 PGj2 Incr23 Sep23 MInj23' injRet23 Fwd2 Unch222' H10 Unch2233' H12 WD2'
+    H14 ValV2 H16).
+  destruct core_after_external23 as [d23' [cc2' [c3' [AftExt22 [AftExt3 MC23']]]]].
+  rewrite AftExt22 in AftExt2. inv AftExt2.
+  exists (d12', Some c2', d23'). exists c1'. exists c3'.
+  split. assumption.
+  split. assumption.
+  exists c2'. exists m2'. exists j12'. exists j23'. auto.
 Qed.
 End INJINJ.
 
@@ -937,8 +911,10 @@ exists st2' : C3,
      clos_trans (core_data12 * option C2 * core_data23)
        (sem_compose_ord_eq_eq core_ord12 core_ord23 C2) d'
        (d12, Some c2, d23)).
-Proof. intros.   destruct (core_diagram12 _ _ _ _ CS1 _ _ MC12) as [c2' [d12' [MC12' Y]]].
-    assert (ZZ: corestep_plus Sem2 Genv2 c2 m1 c2' m1' \/  (c2,m1) = (c2',m1') /\ core_ord12 d12' d12).
+Proof. 
+  intros.   
+  destruct (core_diagram12 _ _ _ _ CS1 _ _ MC12) as [c2' [d12' [MC12' Y]]].
+  assert (ZZ: corestep_plus Sem2 Genv2 c2 m1 c2' m1' \/  (c2,m1) = (c2',m1') /\ core_ord12 d12' d12).
        destruct Y. auto.
        destruct H.
        destruct H. destruct x.
@@ -1000,147 +976,88 @@ Proof. intros.   destruct (core_diagram12 _ _ _ _ CS1 _ _ MC12) as [c2' [d12' [M
     destruct CS2. inv H.
     exists c3. exists (d12',Some c2',d23).
     split. exists c2'.  split. trivial. split; assumption.
-(*    apply extends_refl.
-    inv H4.*)
-(*    split. constructor; auto.*)
     right. split. exists O. simpl; auto.
-                       apply t_step. constructor 1; auto.
+    apply t_step. constructor 1; auto.
 Qed.
 
 Context {F1 C1 V1 F2 C2 V2 F3 C3 V3} 
-       (I :forall F C V : Type, CoreSemantics (Genv.t F V) C mem (list (ident * globdef F V)) -> AST.program F V -> Prop)
-       (Sem1 : CoreSemantics (Genv.t F1 V1) C1 mem (list (ident * globdef F1 V1)))
-       (Sem2 : CoreSemantics (Genv.t F2 V2) C2 mem (list (ident * globdef F2 V2)))
-       (Sem3 : CoreSemantics (Genv.t F3 V3) C3 mem (list (ident * globdef F3 V3)))
-       ExternIdents epts12  epts23 entrypoints13
-       (P1 : AST.program F1 V1) (P2 : AST.program F2 V2) (P3 : AST.program F3 V3) 
-       (ePts12_ok : CompilerCorrectness.entryPts_ok P1 P2 ExternIdents epts12)
-       (e12 : prog_main P1 = prog_main P2)
-       (g12: CompilerCorrectness.GenvHyp P1 P2)       
-       (EPC: entrypoints_compose epts12 epts23 entrypoints13)
-       (EXT1: In (prog_main P1, CompilerCorrectness.extern_func main_sig) ExternIdents)
-       (EXT2: In (prog_main P2, CompilerCorrectness.extern_func main_sig) ExternIdents)
-       (i1: I F1 C1 V1 Sem1 P1)
-       (Eq_init12 : forall m1 : mem,
-            initial_mem Sem1 (Genv.globalenv P1) m1 (prog_defs P1) ->
-            exists m2 : mem, initial_mem Sem2 (Genv.globalenv P2) m2 (prog_defs P2) /\ m1 = m2)
-       (SimEq12 : Forward_simulation_eq.Forward_simulation_equals mem (list (ident * globdef F1 V1))
-                                          (list (ident * globdef F2 V2)) Sem1 Sem2 (Genv.globalenv P1)
-                                          (Genv.globalenv P2) epts12) 
-       (SimEq23 : Forward_simulation_eq.Forward_simulation_equals mem (list (ident * globdef F2 V2))
-                                         (list (ident * globdef F3 V3)) Sem2 Sem3 (Genv.globalenv P2)
-                                         (Genv.globalenv P3) epts23) .
-(*
-Let D12:Type:= Forward_simulation_eq.core_data SimEq12.
-Let D23:Type:= Forward_simulation_eq.core_data SimEq23.
-
-  Let data13 := (Forward_simulation_eq.core_data SimEq12 * (option C2) * Forward_simulation_eq.core_data SimEq23)%type.
-
-  Inductive sem_compose_ord 
-      : (*data13 -> data13 -> Prop :=*)
- (prod (prod (Forward_simulation_eq.core_data SimEq12) (option C2)) (Forward_simulation_eq.core_data SimEq23)) ->
- (prod (prod (Forward_simulation_eq.core_data SimEq12) (option C2)) (Forward_simulation_eq.core_data SimEq23)) -> Prop :=
-
-    | sem_compose_ord1 :
-        forall (d12 d12':Forward_simulation_eq.core_data SimEq12) (c2:C2) (d23:Forward_simulation_eq.core_data SimEq23),
-           Forward_simulation_eq.core_ord SimEq12  d12 d12' ->
-           sem_compose_ord (d12,Some c2,d23) (d12',Some c2,d23)
-    | sem_compose_ord2 :
-        forall (d12 d12':Forward_simulation_eq.core_data SimEq12) (c2 c2':C2) (d23 d23':Forward_simulation_eq.core_data SimEq23),
-           Forward_simulation_eq.core_ord  SimEq23 d23 d23' ->
-           sem_compose_ord (d12,Some c2,d23) (d12',Some c2',d23').
- 
-  Lemma well_founded_sem_compose_ord: well_founded sem_compose_ord. 
-  Proof. 
-    intro. destruct a as [[d12 c2] d23].
-    revert d12. 
-    destruct c2. 
-    2: constructor; intros. 2: inv H.
-(*    set (q := (d23,c)).
-    change d23 with (fst q). change c with (snd q). clearbody q.
-    clear d23.*)
-   revert c. 
-    induction d23 using (well_founded_induction (Forward_simulation_eq.core_ord_wf SimEq23)).
-    intros.
-(*    set (q' := (d12,c)).
-    change d12 with (fst q'). change c with (snd q').
-    clearbody q'. clear d12 c.*)
-    induction d12 using (well_founded_induction (Forward_simulation_eq.core_ord_wf SimEq12)).
-    constructor; intros. inv H1.
-    generalize (H0 d0). simpl. intros.
-    apply H1. auto. (* destruct q'; auto.*) 
-    generalize (H d1). 
-    intros. 
-    spec H1. auto. (* destruct q; auto.*)
-    apply H1. 
-  Qed.
-*)
-(*
-  Lemma well_founded_sem_compose_ord_withmem : well_founded sem_compose_ord.
-  Proof.
-    intro. destruct a as [[d12 [c2 m]] d23].
-    revert d12 m.
-    destruct c2.
-    2: constructor; intros. 2: inv H.
-(*    set (q := (d23,c)).
-    change d23 with (fst q). change c with (snd q). clearbody q.
-    clear d23 c.*)
-   revert c.
-    induction d23 using (well_founded_induction (Forward_simulation_eq.core_ord_wf SimEq23)).
-    intros.
-(*    set (q' := (d12,c)).
-    change d12 with (fst q'). change c with (snd q').
-    clearbody q'. clear d12 c.*)
-    induction d12 using (well_founded_induction (Forward_simulation_eq.core_ord_wf SimEq12)).
-    constructor; intros. inv H1.
-    generalize (H0 d12). simpl. intros.
-    apply H1. auto. (* destruct q'; auto.*)
-    generalize (H d23).
-    intros.
-    spec H1. auto. (* destruct q; auto.*)
-    apply H1.
-  Qed.
-*)
+  (I :forall F C V : Type, 
+    CoreSemantics (Genv.t F V) C mem (list (ident * globdef F V)) -> 
+    AST.program F V -> Prop)
+  (Sem1 : CoreSemantics (Genv.t F1 V1) C1 mem (list (ident * globdef F1 V1)))
+  (Sem2 : CoreSemantics (Genv.t F2 V2) C2 mem (list (ident * globdef F2 V2)))
+  (Sem3 : CoreSemantics (Genv.t F3 V3) C3 mem (list (ident * globdef F3 V3)))
+  ExternIdents epts12  epts23 entrypoints13
+  (P1 : AST.program F1 V1) (P2 : AST.program F2 V2) (P3 : AST.program F3 V3) 
+  (ePts12_ok : CompilerCorrectness.entryPts_ok P1 P2 ExternIdents epts12)
+  (e12 : prog_main P1 = prog_main P2)
+  (g12: CompilerCorrectness.GenvHyp P1 P2)       
+  (EPC: entrypoints_compose epts12 epts23 entrypoints13)
+  (EXT1: In (prog_main P1, CompilerCorrectness.extern_func main_sig) ExternIdents)
+  (EXT2: In (prog_main P2, CompilerCorrectness.extern_func main_sig) ExternIdents)
+  (i1: I F1 C1 V1 Sem1 P1)
+  (Eq_init12 : forall m1 : mem,
+    initial_mem Sem1 (Genv.globalenv P1) m1 (prog_defs P1) ->
+    exists m2 : mem, initial_mem Sem2 (Genv.globalenv P2) m2 (prog_defs P2) /\ m1 = m2)
+  (SimEq12 : Forward_simulation_eq.Forward_simulation_equals mem (list (ident * globdef F1 V1))
+    (list (ident * globdef F2 V2)) Sem1 Sem2 (Genv.globalenv P1)
+    (Genv.globalenv P2) epts12) 
+  (SimEq23 : Forward_simulation_eq.Forward_simulation_equals mem (list (ident * globdef F2 V2))
+    (list (ident * globdef F3 V3)) Sem2 Sem3 (Genv.globalenv P2)
+    (Genv.globalenv P3) epts23).
 
 Lemma eqeq: Forward_simulation_eq.Forward_simulation_equals mem (list (ident * globdef F1 V1))
-                                       (list (ident * globdef F3 V3)) Sem1 Sem3 (Genv.globalenv P1)
-                                       (Genv.globalenv P3) entrypoints13.
+  (list (ident * globdef F3 V3)) Sem1 Sem3 (Genv.globalenv P1)
+  (Genv.globalenv P3) entrypoints13.
 Proof.
-         destruct SimEq12 as [core_data12 match_core12 core_ord12 core_ord_wf12 core_diagram12 core_initial12 core_halted12 core_at_external12 core_after_external12].  
-         destruct SimEq23 as [core_data23 match_core23 core_ord23 core_ord_wf23 core_diagram23 core_initial23 core_halted23 core_at_external23 core_after_external23].
-          eapply Forward_simulation_eq.Build_Forward_simulation_equals with
-                 (core_data:= prod (prod core_data12 (option C2)) core_data23) 
-                 (match_core := fun d c1 c3 => match d with (d1,X,d2) => exists c2, X=Some c2 /\ match_core12 d1 c1 c2 /\ match_core23 d2 c2 c3 end)
-                 (core_ord := clos_trans _ (sem_compose_ord_eq_eq core_ord12 core_ord23 C2)).
+  destruct SimEq12 as [core_data12 match_core12 core_ord12 core_ord_wf12 core_diagram12 
+    core_initial12 core_halted12 core_at_external12 core_after_external12].  
+  destruct SimEq23 as [core_data23 match_core23 core_ord23 core_ord_wf23 core_diagram23 
+    core_initial23 core_halted23 core_at_external23 core_after_external23].
+  eapply Forward_simulation_eq.Build_Forward_simulation_equals with
+    (core_data:= prod (prod core_data12 (option C2)) core_data23) 
+    (match_core := fun d c1 c3 => match d with (d1,X,d2) => 
+      exists c2, X=Some c2 /\ match_core12 d1 c1 c2 /\ match_core23 d2 c2 c3 end)
+    (core_ord := clos_trans _ (sem_compose_ord_eq_eq core_ord12 core_ord23 C2)).
            (*wellfounded*) 
-                eapply wf_clos_trans. eapply well_founded_sem_compose_ord_eq_eq; assumption.
+  eapply wf_clos_trans. eapply well_founded_sem_compose_ord_eq_eq; assumption.
            (*core_diagram*) 
-                 clear core_initial23  core_halted23 core_at_external23 core_after_external23 core_initial12  core_halted12 core_at_external12 core_after_external12 Eq_init12 SimEq12 SimEq23
-                          i1 I core_ord_wf23 core_ord_wf12 EXT2 EXT1 EPC e12 g12 ePts12_ok epts12  epts23 entrypoints13.
-                 intros. destruct d as [[d12 cc2] d23]. destruct H0 as [c2 [X [? ?]]]; subst.
-                 eapply (diagram_eqeq _ _ _ _ _ _ _ _ _ Sem1 Sem2 Sem3 core_data12 match_core12 _ _ _ core_diagram12 _ _ _ _ core_diagram23); eassumption. 
+  clear core_initial23  core_halted23 core_at_external23 core_after_external23 core_initial12  
+    core_halted12 core_at_external12 core_after_external12 Eq_init12 SimEq12 SimEq23
+    i1 I core_ord_wf23 core_ord_wf12 EXT2 EXT1 EPC e12 g12 ePts12_ok epts12  epts23 entrypoints13.
+  intros. destruct d as [[d12 cc2] d23]. destruct H0 as [c2 [X [? ?]]]; subst.
+  eapply (diagram_eqeq _ _ _ _ _ _ _ _ _ Sem1 Sem2 Sem3 
+    core_data12 match_core12 _ _ _ core_diagram12 _ _ _ _ core_diagram23); eassumption. 
            (*initial_core*)
-                  intros. rename v2 into v3. rewrite (EPC v1 v3 sig) in H. destruct H as [v2 [EP12 EP23]].
-                  destruct (core_initial12 _ _ _ EP12 _ H0) as [d12 [c1 [c2 [Ini1 [Ini2 MC12]]]]].
-                  destruct (core_initial23 _ _ _ EP23 _ H0) as [d23 [c22 [c3 [Ini22 [Ini3 MC23]]]]].
-                  rewrite Ini22 in Ini2. inv Ini2.
-                  exists (d12,Some c2,d23). exists c1. exists c3. split; trivial. split; trivial. exists c2. split; trivial. split; trivial.
+  intros. rename v2 into v3. rewrite (EPC v1 v3 sig) in H. destruct H as [v2 [EP12 EP23]].
+  destruct (core_initial12 _ _ _ EP12 _ H0) as [d12 [c1 [c2 [Ini1 [Ini2 MC12]]]]].
+  destruct (core_initial23 _ _ _ EP23 _ H0) as [d23 [c22 [c3 [Ini22 [Ini3 MC23]]]]].
+  rewrite Ini22 in Ini2. inv Ini2.
+  exists (d12,Some c2,d23). exists c1. exists c3. split; trivial. split; trivial. 
+    exists c2. split; trivial. split; trivial.
            (*safely_halted*)
-                    intros. rename c2 into c3. destruct cd as [[d12 cc2] d23]. destruct H as [c2 [X [MC12 MC23]]]. subst.
-                    apply (core_halted12 _ _ _ _ MC12) in H0.
-                    apply (core_halted23 _ _ _ _ MC23) in H0. assumption.
+  intros. rename c2 into c3. destruct cd as [[d12 cc2] d23]. 
+    destruct H as [c2 [X [MC12 MC23]]]. subst.
+  apply (core_halted12 _ _ _ _ MC12) in H0.
+  apply (core_halted23 _ _ _ _ MC23) in H0. assumption.
            (*atexternal*)
-                    intros. rename st2 into st3. destruct d as [[d12cc2]  d23]. destruct H as [st2 [X [MC12 MC23]]]; subst.
-                    apply (core_at_external12 _ _ _ _ _ _ MC12) in H0. destruct H0.
-                    apply (core_at_external23 _ _ _ _ _ _ MC23) in H. assumption.  
+  intros. rename st2 into st3. destruct d as [[d12cc2]  d23]. 
+    destruct H as [st2 [X [MC12 MC23]]]; subst.
+  apply (core_at_external12 _ _ _ _ _ _ MC12) in H0. destruct H0.
+  apply (core_at_external23 _ _ _ _ _ _ MC23) in H. assumption.  
           (*after_external*)
-                    intros. rename st2 into st3. destruct d as [[d12 cc2] d23]. destruct H as [st2 [X [MC12 MC23]]]; subst.
-                    destruct (core_at_external12 _ _ _ _ _ _ MC12 H0)  as [AtExt2 _].
-                    destruct (core_after_external12 _ _ _ _ _ _ _ MC12 H0 AtExt2 H2 H3) as [c1' [c2' [d12' [AftExt1 [AftExt2 MS12']]]]].
-                    destruct (core_after_external23 _ _ _ _ _ _ _ MC23 AtExt2 H1 H2 H3) as [c22' [c3' [d23' [AftExt22 [AftExt3 MS23']]]]].
-                    rewrite AftExt22 in AftExt2. inv AftExt2.
-                    exists c1'. exists c3'. exists (d12',Some c2',d23'). split; trivial. split; trivial. exists c2'. split; trivial. split; trivial. 
+  intros. rename st2 into st3. destruct d as [[d12 cc2] d23]. 
+    destruct H as [st2 [X [MC12 MC23]]]; subst.
+  destruct (core_at_external12 _ _ _ _ _ _ MC12 H0)  as [AtExt2 _].
+  destruct (core_after_external12 _ _ _ _ _ _ _ MC12 H0 AtExt2 H2 H3) 
+    as [c1' [c2' [d12' [AftExt1 [AftExt2 MS12']]]]].
+  destruct (core_after_external23 _ _ _ _ _ _ _ MC23 AtExt2 H1 H2 H3) 
+    as [c22' [c3' [d23' [AftExt22 [AftExt3 MS23']]]]].
+  rewrite AftExt22 in AftExt2. inv AftExt2.
+  exists c1'. exists c3'. exists (d12',Some c2',d23'). split; trivial. 
+    split; trivial. exists c2'. split; trivial. split; trivial. 
 Qed.
+
 End EQEQ.
 
 Section EQEXT.
@@ -1268,11 +1185,8 @@ Proof. intros.   destruct (core_diagram12 _ _ _ _ CS1 _ _ MC12) as [st2' [d12' [
     destruct CS2. inv H.
     exists st3. exists m3. exists (d12',Some st2',d23).
     split. exists st2'.  split. trivial. split; assumption.
-(*    apply extends_refl.
-    inv H4.*)
-(*    split. constructor; auto.*)
     right. split. exists O. simpl; auto.
-                       apply t_step. constructor 1; auto.
+    apply t_step. constructor 1; auto.
 Qed.
 
 Context {F1 C1 V1 F2 C2 V2 F3 C3 V3} 
@@ -1303,57 +1217,59 @@ Lemma eqext: Coop_forward_simulation_ext.Forward_simulation_extends (list (ident
                                            (list (ident * globdef F3 V3)) Sem1 Sem3 (Genv.globalenv P1)
                                            (Genv.globalenv P3) entrypoints13.
 Proof.
-         destruct SimEq12 as [core_data12 match_core12 core_ord12 core_ord_wf12 
-                          core_diagram12 core_initial12 core_halted12 core_at_external12 core_after_external12].  
-         destruct SimExt23 as [core_data23 match_core23 core_ord23 core_ord_wf23 match_memwd23 match_validblocks23
-                core_diagram23 core_initial23 core_halted23 core_at_external23 core_after_external23].
-           eapply Coop_forward_simulation_ext.Build_Forward_simulation_extends with
-                 (match_state := fun d c1 m1 c3 m3 => match d with (d1,X,d2) => exists c2, X = Some c2 /\ match_core12 d1 c1 c2 /\ match_core23 d2 c2 m1 c3 m3 end)
-                 (core_data:= prod (prod core_data12 (option C2)) core_data23)
-                 (core_ord := clos_trans _ (sem_compose_ord_eq_eq core_ord12 core_ord23 C2)). 
+  destruct SimEq12 as [core_data12 match_core12 core_ord12 core_ord_wf12 
+    core_diagram12 core_initial12 core_halted12 core_at_external12 core_after_external12].  
+  destruct SimExt23 as [core_data23 match_core23 core_ord23 core_ord_wf23 match_memwd23 match_validblocks23
+    core_diagram23 core_initial23 core_halted23 core_at_external23 core_after_external23].
+  eapply Coop_forward_simulation_ext.Build_Forward_simulation_extends with
+    (match_state := fun d c1 m1 c3 m3 => match d with (d1,X,d2) => 
+       exists c2, X = Some c2 /\ match_core12 d1 c1 c2 /\ match_core23 d2 c2 m1 c3 m3 end)
+    (core_data:= prod (prod core_data12 (option C2)) core_data23)
+    (core_ord := clos_trans _ (sem_compose_ord_eq_eq core_ord12 core_ord23 C2)). 
            (*well_founded*)
-                 eapply wf_clos_trans. eapply well_founded_sem_compose_ord_eq_eq; assumption.
+  eapply wf_clos_trans. eapply well_founded_sem_compose_ord_eq_eq; assumption.
             (*match_wd*) intros. rename c2 into c3.  rename m2 into m3. destruct d as [[d12 cc2] d23]. 
-                         destruct H as [c2 [X [MC12 MC23]]]; subst.
-                         apply (match_memwd23 _ _ _ _ _ MC23).
+  destruct H as [c2 [X [MC12 MC23]]]; subst.
+  apply (match_memwd23 _ _ _ _ _ MC23).
             (*match_validblocks*) intros. rename c2 into c3.  rename m2 into m3. destruct d as [[d12 cc2] d23]. 
-                         destruct H as [c2 [X [MC12 MC23]]]; subst.
-                         eapply (match_validblocks23 _ _ _ _ _ MC23); try eassumption.
+  destruct H as [c2 [X [MC12 MC23]]]; subst.
+  eapply (match_validblocks23 _ _ _ _ _ MC23); try eassumption.
            (*core_diagram*) 
-                 clear core_initial23  core_halted23 core_at_external23 core_after_external23 core_initial12  core_halted12 core_at_external12 core_after_external12
-                          i1 I core_ord_wf23 core_ord_wf12 EXT2 EXT1 EPC e12 g12 ePts12_ok epts12  epts23 entrypoints13 Eq_init12 SimEq12 SimExt23.
-                 intros. rename st2 into st3.
-                 destruct cd as [[d12 cc2] d23]. destruct H0 as [st2 [X [? ?]]]; subst. rename m2 into m3.
-                 eapply (diagram_eqext _ _ _ _ _ _ _ _ _ Sem1 Sem2 Sem3 core_data12 match_core12 _ _ _ core_diagram12 _ _ _ _ core_diagram23); eassumption. 
+  clear core_initial23  core_halted23 core_at_external23 core_after_external23 core_initial12  core_halted12 core_at_external12 core_after_external12
+    i1 I core_ord_wf23 core_ord_wf12 EXT2 EXT1 EPC e12 g12 ePts12_ok epts12  epts23 entrypoints13 Eq_init12 SimEq12 SimExt23.
+  intros. rename st2 into st3.
+  destruct cd as [[d12 cc2] d23]. destruct H0 as [st2 [X [? ?]]]; subst. rename m2 into m3.
+  eapply (diagram_eqext _ _ _ _ _ _ _ _ _ Sem1 Sem2 Sem3 core_data12 match_core12 _ _ _ core_diagram12 _ _ _ _ core_diagram23); eassumption. 
            (*initial_core*)
-                  intros. rename v2 into v3. rewrite (EPC v1 v3 sig) in H. destruct H as [v2 [EP12 EP23]].
-                  assert (HT: Forall2 Val.has_type vals (sig_args sig)). eapply forall_lessdef_hastype; eauto.
-                  destruct (core_initial12 _ _ _ EP12 _ HT) as [d12 [c1 [c2 [Ini1 [Ini2 MC12]]]]].
-                  destruct (core_initial23 _ _ _ EP23 _ _ _ _ H0 H1 H2 H3 H4) as [d23 [c22 [c3 [Ini22 [Ini3 MC23]]]]].
-                  rewrite Ini22 in Ini2. inv Ini2.
-                  exists (d12,Some c2,d23). exists c1. exists c3. 
-                  split; trivial. split; trivial. exists c2. split; trivial. split; trivial.
+  intros. rename v2 into v3. rewrite (EPC v1 v3 sig) in H. destruct H as [v2 [EP12 EP23]].
+  assert (HT: Forall2 Val.has_type vals (sig_args sig)). eapply forall_lessdef_hastype; eauto.
+  destruct (core_initial12 _ _ _ EP12 _ HT) as [d12 [c1 [c2 [Ini1 [Ini2 MC12]]]]].
+  destruct (core_initial23 _ _ _ EP23 _ _ _ _ H0 H1 H2 H3 H4) as [d23 [c22 [c3 [Ini22 [Ini3 MC23]]]]].
+  rewrite Ini22 in Ini2. inv Ini2.
+  exists (d12,Some c2,d23). exists c1. exists c3. 
+  split; trivial. split; trivial. exists c2. split; trivial. split; trivial.
            (*safely_halted*)
-                    intros. rename st2 into c3. destruct cd as [[d12 cc2] d23]. destruct H as [c2 [X [MC12 MC23]]]; subst.
-                    apply (core_halted12 _ _ _ _ MC12) in H0.
-                    apply (core_halted23 _ _ _ _ _ _ MC23) in H0. assumption. assumption.
+  intros. rename st2 into c3. destruct cd as [[d12 cc2] d23]. destruct H as [c2 [X [MC12 MC23]]]; subst.
+  apply (core_halted12 _ _ _ _ MC12) in H0.
+  apply (core_halted23 _ _ _ _ _ _ MC23) in H0. assumption. assumption.
            (*atexternal*)
-                    intros. rename st2 into st3. destruct cd as [[d12 cc2] d23]. destruct H as [st2 [X [MC12 MC23]]].
-                    apply (core_at_external12 _ _ _ _ _ _ MC12) in H0. destruct H0.
-                    apply (core_at_external23 _ _ _ _ _ _ _ _ MC23) in H. assumption. assumption.
+  intros. rename st2 into st3. destruct cd as [[d12 cc2] d23]. destruct H as [st2 [X [MC12 MC23]]].
+  apply (core_at_external12 _ _ _ _ _ _ MC12) in H0. destruct H0.
+  apply (core_at_external23 _ _ _ _ _ _ _ _ MC23) in H. assumption. assumption.
            (*after_external*)
-                    intros. rename st2 into st3. destruct cd as [[d12 cc2] d23]. destruct H as [st2 [X [MC12 MC23]]].
-                    destruct (core_at_external12 _ _ _ _ _ _ MC12 H0)  as [AtExt2 _].
-                    assert (HVals1:  Forall2 Val.has_type vals1 (sig_args ef_sig)). eapply forall_lessdef_hastype; eauto.
-                    assert (HRet1:   Val.has_type ret1 (proj_sig_res ef_sig)). eapply lessdef_hastype; eauto.
-                    destruct (core_after_external12 _ _ _ _ _ _ _ MC12 H0 AtExt2 HVals1 HRet1) 
-                        as [c1' [c2' [d12' [AftExt1 [AftExt2 MS12']]]]].
-                    destruct (core_after_external23 _ _ _ _ _ _ _ _ _ _ _ _ _ MC23 AtExt2 H1 H2 H3 H4 H5 H6 H7 H8 H9 
-                        H10 H11 H12 H13 H14) as [c22' [c3' [d23' [AftExt22 [AftExt3 MS23']]]]].
-                    rewrite AftExt22 in AftExt2. inv AftExt2.
-                    exists c1'. exists c3'. exists (d12',Some c2',d23'). 
-                    split; trivial. split; trivial. exists c2'. split; trivial. split; trivial.
+  intros. rename st2 into st3. destruct cd as [[d12 cc2] d23]. destruct H as [st2 [X [MC12 MC23]]].
+  destruct (core_at_external12 _ _ _ _ _ _ MC12 H0)  as [AtExt2 _].
+  assert (HVals1:  Forall2 Val.has_type vals1 (sig_args ef_sig)). eapply forall_lessdef_hastype; eauto.
+  assert (HRet1:   Val.has_type ret1 (proj_sig_res ef_sig)). eapply lessdef_hastype; eauto.
+  destruct (core_after_external12 _ _ _ _ _ _ _ MC12 H0 AtExt2 HVals1 HRet1) 
+    as [c1' [c2' [d12' [AftExt1 [AftExt2 MS12']]]]].
+  destruct (core_after_external23 _ _ _ _ _ _ _ _ _ _ _ _ _ MC23 AtExt2 H1 H2 H3 H4 H5 H6 H7 H8 H9 
+    H10 H11 H12 H13 H14) as [c22' [c3' [d23' [AftExt22 [AftExt3 MS23']]]]].
+  rewrite AftExt22 in AftExt2. inv AftExt2.
+  exists c1'. exists c3'. exists (d12',Some c2',d23'). 
+  split; trivial. split; trivial. exists c2'. split; trivial. split; trivial.
 Qed.
+
 End EQEXT.
 
 Section EQINJ.
@@ -1507,9 +1423,6 @@ Proof. intros.
     split. apply inject_incr_refl.
     split. apply inject_separated_same_meminj. 
     split. exists st2'.  split. trivial. split; assumption.
-(*    apply extends_refl.
-    inv H4.*)
-(*    split. constructor; auto.*)
     right. split. exists O. simpl; auto.
                        apply t_step. constructor 1; auto.
 Qed.
@@ -2872,406 +2785,6 @@ Proof.
                     exists c2'. exists m2'.  split; trivial. split; assumption.
 Qed.
 End INJEXT.
-
-(*
-Section INJINJFULL.
-
-Lemma diagram_injinjfull: forall
-(G1 C1 D1 : Type)
-(G2 C2 D2 : Type)
-(G3 C3 D3 : Type)
-(Sem1 : CoreSemantics G1 C1 mem D1)
-(Sem2 : CoreSemantics G2 C2 mem D2)
-(Sem3 : CoreSemantics G3 C3 mem D3)
-(core_data12 : Type)
-(match_core12 : core_data12 -> meminj -> C1 -> mem -> C2 -> mem -> Prop)
-(core_ord12 : core_data12 -> core_data12 -> Prop)
-(Genv2 : G2)
-(Genv1 : G1)
-(core_diagram12 : forall (st1 : C1) (m1 : mem) (st1' : C1) (m1' : mem),
-                 corestep Sem1 Genv1 st1 m1 st1' m1' ->
-                 forall (cd : core_data12) (st2 : C2) (j : meminj) (m2 : mem),
-                 match_core12 cd j st1 m1 st2 m2 ->
-                 exists st2' : C2,
-                   exists m2' : mem,
-                     exists cd' : core_data12,
-                       exists j' : meminj,
-                         inject_incr j j' /\
-                         inject_separated j j' m1 m2 /\
-                         match_core12 cd' j' st1' m1' st2' m2' /\
-                         (corestep_plus Sem2 Genv2 st2 m2 st2' m2' \/
-                          corestep_star Sem2 Genv2 st2 m2 st2' m2' /\ core_ord12 cd' cd))
-(core_data23 : Type)
-(match_core23 : core_data23 -> meminj -> C2 -> mem -> C3 -> mem -> Prop)
-(core_ord23 : core_data23 -> core_data23 -> Prop)
-(Genv3 : G3)
-(core_diagram23 : forall (st1 : C2) (m1 : mem) (st1' : C2) (m1' : mem),
-                   corestep Sem2 Genv2 st1 m1 st1' m1' ->
-                   forall (cd : core_data23) (st2 : C3) 
-                     (j : meminj) (m2 : mem),
-                   match_core23 cd j st1 m1 st2 m2 ->
-                   exists st2' : C3,
-                     exists m2' : mem,
-                       exists cd' : core_data23,
-                         exists j' : meminj,
-                           inject_incr j j' /\
-                           inject_separated j j' m1 m2 /\
-                           match_core23 cd' j' st1' m1' st2' m2' /\
-                           (corestep_plus Sem3 Genv3 st2 m2
-                              st2' m2' \/
-                            corestep_star Sem3 Genv3 st2 m2
-                              st2' m2' /\ core_ord23 cd' cd))
- (st1 : C1)
-  (m1 : mem)
-  (st1' : C1)
-  (m1' : mem)
-  (CS1 : corestep Sem1 Genv1 st1 m1 st1' m1')
-  (d12 : core_data12)
-  (d23 : core_data23)
-  (st3 : C3)
-  (m3 : mem)
-  (st2 : C2)
-  (m2 : mem)
-  (j12 : meminj)
-  (j23 : meminj)
-  (BV12: forall b1 b2 ofs, j12 b1 = Some (b2,ofs) -> Mem.valid_block m1 b1 /\ Mem.valid_block m2 b2)
-  (BV23: forall b2 b3 ofs, j23 b2 = Some (b3,ofs) -> Mem.valid_block m2 b2 /\ Mem.valid_block m3 b3)
-  (MC12 : match_core12 d12 j12 st1 m1 st2 m2)
-  (MC23 : match_core23 d23 j23 st2 m2 st3 m3)
-  (CSF2 : corestep_fwd Sem2)
-  (CSF3 : corestep_fwd Sem3),
-   exists st2' : C3,
-     exists m2' : mem,
-       exists cd' : core_data12 * option C2 * core_data23,
-         exists j' : meminj,
-           inject_incr (compose_meminj j12 j23) j' /\
-           inject_separated (compose_meminj j12 j23) j' m1 m3 /\
-           (let (y, d2) := cd' in
-            let (d1, X) := y in
-            exists c2 : C2,
-              exists m0 : mem,
-                exists j1 : meminj,
-                  exists j2 : meminj,
-                    X = Some c2 /\
-                    j' = compose_meminj j1 j2 /\
-                    match_core12 d1 j1 st1' m1' c2 m0 /\
-                    match_core23 d2 j2 c2 m0 st2' m2') /\
-           (corestep_plus Sem3 Genv3 st3 m3 st2' m2' \/
-            corestep_star Sem3 Genv3 st3 m3 st2' m2' /\
-            clos_trans (core_data12 * option C2 * core_data23)
-              (sem_compose_ord_eq_eq core_ord12 core_ord23 C2) cd'
-              (d12, Some st2, d23)).
-Proof. intros. 
-    destruct (core_diagram12 _ _ _ _ CS1 _ _ _ _ MC12)
-          as [st2' [m2' [d12' [j12' [InjIncr12 
-                    [InjSep12 [MC12' Y]]]]]]]; clear core_diagram12.
-    assert (ZZ: corestep_plus Sem2 Genv2 st2 m2 st2' m2' \/
-                 (st2,m2) = (st2',m2') /\ core_ord12 d12' d12).
-       destruct Y. auto.
-       destruct H.
-       destruct H. destruct x.
-       right. split; auto.
-       left. exists x; auto.
-    clear Y. destruct ZZ as [CS2 | CS2 ord12'].
- (*case1*) 
-    destruct CS2.
-    clear MC12 CS1. 
-    assert (exists mm2, exists jj,
-           corestepN Sem2 Genv2 (S x) st2 mm2 st2' m2' /\ 
-                       mem_forward m2 mm2 /\
-                        match_core23 d23 jj st2 mm2 st3 m3 /\
-            inject_incr j23 jj /\
-           forall (b2 b3 : block) (ofs : Z),
-             jj b2 = Some (b3, ofs) ->
-             Mem.valid_block m2 b2 /\ Mem.valid_block m3 b3).
-           exists m2. exists j23. split; trivial. 
-               split. apply mem_forward_refl. 
-               split. trivial. split. apply inject_incr_refl.  auto.
-    clear H MC23 BV23.
-    destruct H0 as [mm2 [jj [H [Y2 [MC23 [JJ BV23]]]]]]. 
-    revert j23 d23 st2 mm2 st3 H Y2 JJ MC23. 
-    induction x; intros. 
-      (*base case*) simpl in H.
-          destruct H as [c2 [m2'' [? ?]]].
-          inv H0.
-          destruct (core_diagram23 _ _ _ _ H _ _ _ _ MC23) as [st3' [m3' [d23' [j23' [InjInc23 [InjSep23 [? ?]]]]]]].
-          exists st3'. exists m3'. exists (d12',Some st2',d23'). 
-          exists (compose_meminj j12' j23').
-          split. eapply  compose_meminj_inject_incr; try eassumption.
-                  eapply inject_incr_trans; eassumption.
-          split. intros b; intros.
-                apply compose_meminjD_Some in H3. 
-                destruct H3 as [b1 [ofs1 [ofs [Hb [Hb1 DD]]]]]; subst.
-                apply compose_meminjD_None in H2.
-                destruct H2.
-                  destruct (InjSep12 _ _ _ H2 Hb).
-                  split; trivial. 
-                  remember (j23 b1) as z. 
-                  destruct z; apply eq_sym in Heqz.
-                     destruct p. specialize (JJ _ _ _ Heqz). 
-                         specialize (InjInc23 _ _ _ JJ). 
-                         rewrite InjInc23 in Hb1. inv Hb1. 
-                         destruct (BV23 _ _ _ Heqz).
-                         exfalso. apply (H4 H5).
-                  remember (jj b1) as zz.
-                  destruct zz; apply eq_sym in Heqzz.
-                     destruct p. specialize (InjInc23 _ _ _ Heqzz).
-                       rewrite InjInc23 in Hb1. inv Hb1.
-                  destruct (InjSep23 _ _ _ Heqz Hb1). apply H6.
-                destruct H2 as [b22 [ofs22 [XX YY]]].
-                    specialize (InjIncr12 _ _ _ XX). rewrite InjIncr12 in Hb. inv Hb.
-                   destruct (InjSep23 _ _ _ YY Hb1).
-                    split; trivial. 
-                    destruct (BV12 _ _ _ XX).
-                    apply Y in H5. exfalso. apply H2. apply H5.
-          split. exists st2'. exists m2'. exists j12'. exists j23'.
-            auto. 
-          destruct H1. left; assumption.
-          destruct H1. right. split; trivial.
-          apply t_step. constructor 2. apply H2.
-     (*inductive case*)
-           remember (S x) as x'. simpl in H.
-           destruct H as [st2'' [m2'' [? ?]]]. subst x'.
-           destruct (core_diagram23 _ _ _ _  H _ _ _ _ MC23) as [c3' [m3' [d23' [j23' [InjInc23 [InjSep23 [? ?]]]]]]]. clear core_diagram23.
-           specialize (IHx _ _ _ _ _ H1 MC12' H0).
-           assert (BV23': forall (b2 b3 : block) (ofs : Z),
-         j23' b2 = Some (b3, ofs) ->
-         Mem.valid_block m2 b2 /\ Mem.valid_block m3' b3). 
-                clear IHx. intros.
-                remember (j23 b2) as z. 
-                destruct z; apply eq_sym in Heqz. 
-                   destruct p. specialize (InjInc23 _ _ _ Heqz). 
-                      rewrite InjInc23 in H3.  inv H3. 
-                   destruct (BV23 _ _ _ Heqz). split; trivial. admit. (*by CSF3*)
-                destruct (InjSep23 _ _ _ Heqz H3). 
-                  split; trivial. 
-                  assert (Mem.inject j23' m2'' m3'). admit. (*From H1*)
-                  apply (Mem.valid_block_inject_1 _ _ _ _ _ _ H3) in H6.                 apply Y 
-                 SearchAbout Mem.inject.  Mem.inject_block_valid_1. 
-                  (*by H1*)
-           assert (Sep: inject_separated j12 j12' m1 m2'').
-              clear IHx. intros b; intros.
-              destruct (InjSep12 _ _ _ H3 H4).
-              split; trivial.
-              intros N. apply H6.
-assert (BV12': forall (b1 b2 : block) (ofs : Z), j12' b1 = Some (b2, ofs) ->
-                           Mem.valid_block m1' b1 /\ Mem.valid_block m2'' b2).
-               intros. apply BV12 in H3. destruct 
-               admit. (*from MC
-              clear IHx. intros. 
-              remember (j12 b1) as z. 
-              destruct z; apply eq_sym in Heqz. 
-                destruct p. rewrite (InjIncr12 _ _ _ Heqz) in H3. inv H3. destruct (BV12 _ _ _ Heqz).
-                split; trivial. eapply CSF2. apply H. apply H4.
-                destruct (InjSep12 _ _ _ Heqz H3).
-           assert (BV23': forall (b2 b3 : block) (ofs : Z), j23' b2 = Some (b3, ofs) ->
-                          Mem.valid_block m2'' b2 /\ Mem.valid_block m3' b3).
-              clear IHx. intros. admit. (*From H1: match23 m2'' m3'*) 
-           assert (InjSep'': inject_separated j12 j12' m1 m2'').
-              clear IHx core_diagram23. intros b; intros. 
-                  destruct (InjSep12 _ _ _ H3 H4). split; trivial.
-                  remember (j23 b2) as z.
-                  destruct z; apply eq_sym in Heqz.
-                    destruct p. apply BV23 in Heqz. exfalso. apply H6. apply Heqz.   
-                  remember (j23' b2) as zz.
-                  destruct zz; apply eq_sym in Heqzz.
-                    destruct p. destruct (BV23' _ _ _ Heqzz). apply BV23 in Heqz. exfalso. apply H6. apply Heqz.                  
-                  intros N. apply H6.
-SearchAbout inject_separated.xx
-              remember (j23 b2) as j23b2. 
-              destruct j23b2; apply eq_sym in Heqj23b2. 
-              (*Some*) destruct p. assert (XX:= InjInc23 _ _ _ Heqj23b2). rewrite H3 in XX. inv XX.
-                       destruct (BV23 _ _ _ Heqj23b2).
-                       split. eapply CSF2. apply H. apply H4.
-                       destruct H2 as [H2 | [H2 _]]. 
-                         eapply (corestep_plus_fwd _ CSF3 _ _ _ _ _ H2 _ H5). 
-                         eapply (corestep_star_fwd _ CSF3 _ _ _ _ _ H2 _ H5).
-              (*None*)  eapply CSF3. apply H. apply H4.
-              split; trivial. eapply CSF2. apply H. apply H5.
-                  
-           assert (YY:  forall b : block, Mem.valid_block m1 b -> Mem.valid_block m2'' b) .
-              intros. clear IHx. apply BV12 in H3. apply CSF2 in H. eapply H. apply H3.
-           specialize (IHx _ _ _ _ _ _ _ _ H1 MC12' H0 YY).
-           destruct IHx as [c3'' [m3'' [[[d12''' cc2''] d23'']  [j'' [InjIncr' [InjSep' [[c2'' [m2''' [X [MC12'' MC23'']]]] ?]]]]]]]. subst.
-           exists c3''. exists m3''. exists (d12''', Some c2'',d23''). exists j''.
-           split. eapply inject_incr_trans; eassumption.
-           split. intros b. intros.
-                     remember (j' b) as jb.
-                     destruct jb; apply eq_sym in Heqjb.
-                          destruct p. rewrite (InjIncr' _ _ _ Heqjb) in H5. inv H5. 
-                                   destruct (InjSep _ _ _ H4 Heqjb).
-                                   split; trivial.
-                                   intros N. apply H5. eapply BV12; eassumption. 
-                     destruct (InjSep' _ _ _ Heqjb H5).
-                                   split; trivial.
-                                   intros N. apply H7. 
-                                   destruct H2 as [HH | [HH _]].
-                                      eapply corestep_plus_fwd. apply CSF3. apply HH. assumption.  
-                                      eapply corestep_star_fwd. apply CSF3. apply HH. assumption.  
-           split. exists c2''. exists m2'''. auto.
-           (*inv H8. constructor. auto.
-           split. auto.*)
-           destruct H2; destruct H3.
-           (*1/4*)
-              left. destruct H2 as [n1 ?]. destruct H3 as [n2 ?].
-                      exists (n1 + S n2)%nat.
-                      change (S (n1 + S n2)) with (S n1 + S n2)%nat.
-                      rewrite corestepN_add. eauto.
-           (*2/4*)
-               destruct H3.
-               left. destruct H2 as [n1 ?]. destruct H3 as [n2 ?].
-                       exists (n1 + n2)%nat.
-                       change (S (n1 + n2)) with (S n1 + n2)%nat.
-                       rewrite corestepN_add. eauto.
-           (*3/4*)
-               left. destruct H2.
-                       destruct H2 as [n1 ?]. destruct H3 as [n2 ?].
-                       exists (n1 + n2)%nat.
-                       replace (S (n1 + n2)) with (n1 + S n2)%nat by omega.
-                       rewrite corestepN_add. eauto.
-           (*3/4*)
-               right. destruct H2. destruct H3.
-               split. destruct H2 as [n1 ?]. destruct H3 as [n2 ?].
-                         exists (n1 + n2)%nat.
-                         rewrite corestepN_add. eauto.
-              eapply t_trans; eauto.
-          (*4/4*)
-              apply t_step.
-              constructor 2. apply H4.
-  (*case 2*)
-    destruct CS2. inv H.
-    exists st3. exists m3. exists (d12',Some st2',d23). exists j.
-    split. apply inject_incr_refl.
-    split. apply inject_separated_same_meminj.
-    split. exists st2'. exists m2'. split. trivial. split; assumption.
-(*    apply extends_refl.
-    inv H4.*)
-(*    split. constructor; auto.*)
-    right. split. exists O. simpl; auto.
-                       apply t_step. constructor 1; auto.
-*)
-Qed.
-
-Context {F1 C1 V1 F2 C2 V2 F3 C3 V3} 
-       (I :forall F C V : Type, CoreSemantics (Genv.t F V) C mem (list (ident * globdef F V)) -> AST.program F V -> Prop)
-       (Sem1 : CoreSemantics (Genv.t F1 V1) C1 mem (list (ident * globdef F1 V1)))
-       (Sem2 : CoreSemantics (Genv.t F2 V2) C2 mem (list (ident * globdef F2 V2)))
-       (Sem3 : CoreSemantics (Genv.t F3 V3) C3 mem (list (ident * globdef F3 V3)))
-       ExternIdents epts12  epts23 entrypoints13
-       (P1 : AST.program F1 V1) (P2 : AST.program F2 V2) (P3 : AST.program F3 V3) 
-       (ePts12_ok : CompilerCorrectness.entryPts_ok P1 P2 ExternIdents epts12)
-       (e12 : prog_main P1 = prog_main P2)
-       (g12: CompilerCorrectness.GenvHyp P1 P2)       
-       (EPC: entrypoints_compose epts12 epts23 entrypoints13)
-       (EXT1: In (prog_main P1, CompilerCorrectness.extern_func main_sig) ExternIdents)
-       (EXT2: In (prog_main P2, CompilerCorrectness.extern_func main_sig) ExternIdents)
-       (i1: I F1 C1 V1 Sem1 P1)
-(*       (Inj_init12 : forall m1 : mem,
-               initial_mem Sem1 (Genv.globalenv P1) m1 (prog_defs P1) ->
-               exists m2 : mem,
-                 initial_mem Sem2 (Genv.globalenv P2) m2 (prog_defs P2) /\
-                 Mem.inject j12 m1 m2)*)
-     (SimInj12 : Sim_inj.Forward_simulation_inject (list (ident * globdef F1 V1))
-             (list (ident * globdef F2 V2)) Sem1 Sem2 (Genv.globalenv P1) (Genv.globalenv P2) epts12)
-     (SimInj23 : Sim_inj.Forward_simulation_inject (list (ident * globdef F2 V2))
-             (list (ident * globdef F3 V3)) Sem2 Sem3 (Genv.globalenv P2) (Genv.globalenv P3) epts23)
-     (CSF2: corestep_fwd Sem2) (CSF3: corestep_fwd Sem3).
-
-Lemma injinj: Sim_inj.Forward_simulation_inject (list (ident * globdef F1 V1))
-                                         (list (ident * globdef F3 V3)) Sem1 Sem3 (Genv.globalenv P1)
-                                        (Genv.globalenv P3) entrypoints13.
-Proof.
-  destruct SimInj12 as [core_data12 match_core12 core_ord12 core_ord_wf12 core_diagram12 
-                        core_initial12 core_halted12 core_at_external12 core_after_external12].  
-  destruct SimInj23 as [core_data23 match_core23 core_ord23 core_ord_wf23 core_diagram23 
-                        core_initial23 core_halted23 core_at_external23 core_after_external23].
-  eapply Sim_inj.Build_Forward_simulation_inject with
-                 (core_ord := clos_trans _ (sem_compose_ord_eq_eq core_ord12 core_ord23 C2))
-                 (match_state := fun d j c1 m1 c3 m3 => 
-                    match d with (d1,X,d2) => 
-                        exists c2, exists m2, exists j1, exists j2, 
-                           X=Some c2 /\ j = compose_meminj j1 j2 /\
-                           match_core12 d1 j1 c1 m1 c2 m2 /\ match_core23 d2 j2 c2 m2 c3 m3 
-                                                                                     
-                    end).
-            (*well_founded*)
-                 eapply wf_clos_trans. eapply well_founded_sem_compose_ord_eq_eq; assumption.
-            (*core_diagram*)
-                 clear core_initial23  core_halted23 core_at_external23 core_after_external23 
-                       core_initial12  core_halted12 core_at_external12 core_after_external12
-                       i1 I core_ord_wf23 core_ord_wf12 EXT2 EXT1 EPC e12 g12 ePts12_ok epts12 
-                       epts23 entrypoints13 (*Inj_init12*) SimInj12 SimInj23.
-                 intros. rename st2 into st3. rename m2 into m3.
-                 destruct cd as [[d12 cc2] d23]. destruct H0 as [st2 [m2 [j12 [j23 [X [? [MC12 MC23]]]]]]]; subst.
-              xx   admit. (*eapply (diagram_injinj _ _ _ _ _ _ _ _ _ Sem1 Sem2 Sem3 core_data12 match_core12 _ _ _ 
-                                        core_diagram12 _ _ _ _ core_diagram23); try eassumption.*)
-           (*initial_core*)
-                  intros. rename m2 into m3. rename v2 into v3. rename vals2 into vals3. 
-                  rewrite (EPC v1 v3 sig) in H. destruct H as [v2 [EP12 EP23]].
-                  clear core_at_external12 core_halted12 core_diagram12 core_after_external12
-                        core_at_external23 core_halted23 core_diagram23 core_after_external23.
-                  assert (HT: Forall2 Val.has_type vals1 (sig_args sig)). eapply forall_valinject_hastype; eassumption.
-(*assert (WD1: MEM_WD.mem_wd m1). admit.*)
-                  assert (X: Mem.inject (Mem.flat_inj (Mem.nextblock m1)) m1 m1 /\ 
-                             j = compose_meminj (Mem.flat_inj (Mem.nextblock m1)) j ).
-                      split. apply MEM_WD.mem_wd_E.  admit. (*need  MEM_WD.mem_wd m1*) 
-                             eapply (MEM_WD.meminj_split_flatinjL _ _ _ H1).  admit. (*need  MEM_WD.mem_wd m1*) 
-                  destruct X as [Flat1 XX]. rewrite XX.
-                  assert (ValInjFlat1 := forall_val_inject_flat _ _ _ H1 _ _ H2).
-                  destruct (core_initial12 _ _ _ EP12 _ _ _ _ _ _ H0 Flat1 ValInjFlat1 HT) as [d12 [c2 [Ini2 MC12]]].
-                  destruct (core_initial23 _ _ _ EP23 _ _ _ _ _ _  Ini2 H1 H2 H3) as [d23 [c3 [Ini3 MC23]]].
-                  exists (d12,Some c2,d23). exists c3. 
-                  split; trivial. 
-                  exists c2. exists m1. exists  (Mem.flat_inj (Mem.nextblock m1)). exists j. 
-                  split; trivial. split; trivial. split; assumption.
-             (*safely_halted*)
-                    intros. rename c2 into c3. rename m2 into m3.  
-                    destruct cd as [[d12 cc2] d23]. destruct H as [c2 [m2 [j12 [j23 [X [Y [MC12 MC23]]]]]]]; subst. 
-                    apply (core_halted12 _ _ _ _ _ _ _ MC12) in H0. destruct H0 as [v2 [ValsInj12 [SH2 Minj12]]].
-                    apply (core_halted23 _ _ _ _ _ _ _ MC23) in SH2. destruct SH2 as [v3 [ValsInj23 [SH3 MInj23]]].
-                    exists v3. split. apply (val_inject_compose _ _ _ _ _ ValsInj12 ValsInj23).
-                          split. trivial. eapply Mem.inject_compose; eassumption.
-             (*atexternal*)
-                    intros. rename st2 into st3. rename m2 into m3. 
-                    destruct cd as [[d12 cc2] d23]. 
-                    destruct H as [st2 [m2 [j1 [j2 [Y [J [MC12 MC23]]]]]]]. subst.
-                    apply (core_at_external12 _ _ _ _ _ _ _ _ _ MC12) in H0. 
-                      destruct H0 as [MInj12 [PGj1 [vals2 [ValsInj12 [HTVals2 AtExt2]]]]].
-                    apply (core_at_external23 _ _ _ _ _ _ _ _ _ MC23) in AtExt2. 
-                      destruct AtExt2 as [MInj23 [PGj2 [vals3 [ValsInj23 [HTVals3 AtExt3]]]]].
-                    split. eapply Mem.inject_compose; eassumption.
-                    split. admit. (*need to prove  meminj_preserves_globals (Genv.globalenv P1) (compose_meminj j1 j2)meminj_preserves_globals (Genv.globalenv P1) j1  and meminj_preserves_globals (Genv.globalenv P2) j2*)  
-                    exists vals3. 
-                    split.  eapply forall_val_inject_compose; eassumption.
-                    split; assumption.
-             (*after_external*)
-                    intros. rename st2 into st3. rename m2 into m3. rename ret2 into ret3. rename m2' into m3'. 
-                    destruct cd as [d12 d23]. destruct H0 as [st2 [m2 [j1 [j2 [J [MC12 MC23]]]]]]. subst.
-                    apply (core_at_external12 _ _ _ _ _ _ _ _ _ MC12) in H1. destruct H1 as [MInj12 [PGj1 [vals2 [ValsInj12 [HTVals2 AtExt2]]]]].
-                    apply (core_at_external23 _ _ _ _ _ _ _ _ _ MC23) in AtExt2. destruct AtExt2 as [MInj23 [PGj2 [vals3 [ValsInj23 [HTVals3 AtExt3]]]]].
-                     assert (HVals1:  Forall2 Val.has_type vals1 (sig_args ef_sig)). eapply forall_valinject_hastype; eassumption.
-                    assert (HRet1: Val.has_type ret1 (proj_sig_res ef_sig)). eapply valinject_hastype; eassumption.
-(*Continue here once other pushouts have been proven
-                    destruct (inj_incr_compose_split _ _ _ H3) as [j1' [j2' [Jinc1 [Jinc2 J']]]]. subst. 
-specialize (core_after_external12 cd12 j1 j1' st1 st2 m1 e vals1 ret1 m1' m2 m2'
-                    destruct (pushout_II _ _ j1 MInj12 _ H7 j1') as [m2' [Fwd2 [Ext12' [UnchOn2 X]]]].
-                    destruct (X _ H12) as [UnchOn2j Ext23']; clear X.
-                    destruct (core_after_external12 _ _ _ _ _ _ _ _ ret1 ret1 _ _ _ MC12 H5 AtExt2 
-                            LDVals12 HTVals2 H11 Fwd2 UnchOn2 (Val.lessdef_refl _) Ext12' HRet1) as [c1' [c2' [d12' [AftExt1 [AftExt2 MC12']]]]].
-                    assert (UnchOn3 :  mem_unchanged_on (loc_out_of_reach j m2) m3 m3').
-                        split; intros; eapply H14; trivial.
-                                 eapply extends_loc_out_of_reach; eassumption.
-                                 intros. apply H4 in H17. eapply extends_loc_out_of_reach; eassumption.
-                    specialize (Ext23' _ Inj23 _ H13 H14 _ H7 H8 H9).
-                    assert (Sep23: inject_separated j j' m2 m3).
-                         intros b. intros. destruct (H8 _ _ _ H4 H16). split; trivial. intros N. apply H17.  inv Ext12. unfold Mem.valid_block. rewrite mext_next. apply N.
-                    destruct (core_after_external23 _ j j' _ _ _ _ vals2 ret1 _ _ _ ret3 _ Inj23 MC23 AtExt2 PG2 H7 Sep23 Ext23' H10 Fwd2
-                             UnchOn2j H13 UnchOn3 H15)  as [cc2' [c3' [d23' [AftExt22 [AftExt3 MC23']]]]].
-                    rewrite AftExt22 in AftExt2. inv AftExt2.
-                    exists c1'. exists c3'. exists (d12',d23'). split; trivial. split; trivial. exists c2'. exists m2'.  split; trivial.
-End INJINJ.
-*)
-*)
 
 Lemma cc_trans_CaseInject: forall {F1 C1 V1 F2 C2 V2 F3 C3 V3} 
      (Sem1 : CoopCoreSem (Genv.t F1 V1) C1 (list (ident * globdef F1 V1)))
